compcertox/TensorComp.v
@@ -8,59 +8,6 @@ Require Import Linking.
 Require Import Lifting AbstractStateRel.
 Require Import Coq.Logic.FinFun.
 
-Section Properties.
-
-  Context {K1 K2 K3 K4} (R1: krel K1 K2) (R2: krel K3 K4).
-  Lemma prod_match_reply w r1 r2 k1 k2 k3 k4:
-    match_reply R1 w (r1, k1) (r2, k2) ->
-    Rk R2 k3 k4 -> Rr R2 k3 (cr_mem r2) ->
-    (* kmrel (krel_crel R2) (cr_mem r1, k3) (cr_mem r2, k4) -> *)
-    match_reply (R1 * R2) w (r1, (k1, k3)) (r2, (k2, k4)).
-  Proof.
-    intros [w' [Hw' Hr]] H. exists w'; split.
-    - cbn in *. eapply Mem.unchanged_on_implies; eauto.
-      cbn in *. intros. intro contra. apply H1. now left.
-    - inv Hr. cbn in *. constructor; eauto.
-      + split; eauto.
-      + split; eauto.
-  Qed.
-
-  Lemma prod_match_query w q1 q2 k1 k2 k3 k4:
-    match_query (R1 * R2) w (q1, (k1, k3)) (q2, (k2, k4)) ->
-    match_query R1 w (q1, k1) (q2, k2) /\ Rk R2 k3 k4 /\ Rr R2 k3 w.
-  Proof.
-    intros. inv H. repeat apply conj; cbn in *.
-    constructor; eauto.
-    - intros b ofs Hg. apply H9. now left.
-    - firstorder.
-    - firstorder.
-    - firstorder.
-    - firstorder.
-  Qed.
-
-  Lemma match_query_comm w q1 q2 k1 k2 k3 k4:
-    match_query (R2 * R1) w (q1, (k3, k1)) (q2, (k4, k2)) ->
-    match_query (R1 * R2) w (q1, (k1, k3)) (q2, (k2, k4)).
-  Proof.
-    intros. inv H. constructor; auto.
-    - intros b ofs Hg. apply H9. cbn in *. intuition.
-    - cbn in *. intuition.
-    - cbn in *. intuition.
-  Qed.
-
-  Lemma match_reply_comm w r1 r2 k1 k2 k3 k4:
-    match_reply (R2 * R1) w (r1, (k3, k1)) (r2, (k4, k2)) ->
-    match_reply (R1 * R2) w (r1, (k1, k3)) (r2, (k2, k4)).
-  Proof.
-    intros [w' [Hw H]]. exists w'; split.
-    - cbn in *. eapply Mem.unchanged_on_implies. eauto. cbn. intuition.
-    - inv H. econstructor; auto.
-      + cbn in *. intuition.
-      + cbn in *. intuition.
-  Qed.
-
-End Properties.
-
 Generalizable All Variables.
 
 (* A li_func convert from one language interface to another. This is useful
@@ -321,24 +268,24 @@ End LIFT_COMM.
 Section TENSOR.
 
   Context {K1 K2} (L1: semantics li_null (li_c@K1)) (L2: semantics li_null (li_c@K2)).
-  Context {J1 J2} (jcc: krel J1 J2) (kcc: krel K1 K2).
-  Context (HL: fsim_components 1 kcc L1 L2).
-  Context (se1 se2: Genv.symtbl) (w : ccworld (kcc * jcc)).
-  Context (Hse: match_senv (kcc * jcc) w se1 se2).
+  Context {J1 J2} (jr: krel J1 J2) (kr: krel K1 K2).
+  Context (HL: fsim_components 1 kr L1 L2).
+  Context (se1 se2: Genv.symtbl) (w : ccworld (kr * jr)).
+  Context (Hse: match_senv (kr * jr) w se1 se2).
   Context (Hse1: Genv.valid_for (skel L1) se1).
 
-  Hypothesis Hdisjoint: forall b ofs, G jcc b ofs -> G kcc b ofs -> False.
+  Hypothesis Hdisjoint: forall b ofs, G jr b ofs -> G kr b ofs -> False.
 
   Inductive state_match: fsim_index HL -> state L1 * J1 -> state L2 * J2 -> Prop :=
   | lift_state_match i s1 j1 s2 j2:
       fsim_match_states HL se1 se2 w i s1 s2 ->
-      Rk jcc j1 j2 -> Rr jcc j1 w ->
+      Rk jr j1 j2 -> Rr jr j1 w ->
       state_match i (s1, j1) (s2, j2).
 
   Lemma lift_layer_semantics_simulation:
-    fsim_properties 1 (kcc * jcc) se1 se2 w
-      (lift_layer_k L1 se1) (lift_layer_k L2 se2)
-      (fsim_index HL) (fsim_order HL) state_match.
+    fsim_properties 1 (kr * jr) se1 se2 w
+                    (lift_layer_k L1 se1) (lift_layer_k L2 se2)
+                    (fsim_index HL) (fsim_order HL) state_match.
   Proof.
     split; cbn.
     - intros [q1 [k1 j1]] [q2 [k2 j2]] [s1 sj1] Hq [H Hj]; cbn in *.
@@ -455,93 +402,3 @@ Section INTERC.
   Qed.
 
 End INTERC.
-
-Require Import CModule.
-Require Import Composition.
-Require Import FunctionalExtensionality.
-
-Section TCOMP.
-
-  Context {K1 K2 K3 K4: Type} (R: krel K1 K2) (S: krel K3 K4).
-  Context (L1: layer K1) (L2: layer K2) (L3: layer K3) (L4: layer K4).
-  Context (M N: cmodule).
-
-  Hypothesis (HL1: ksim L1 L2 M R) (HL2: ksim L3 L4 N S).
-  Variable (sk: AST.program unit unit).
-  Hypothesis (Hk1: linkorder (skel L1) sk) (Hk2: linkorder (skel L3) sk).
-  Let Mi := (fun i : bool => if i then semantics M sk else semantics N sk).
-  Context `{!FlatLinkable Mi}.
-  Hypothesis Hdisjoint: forall b ofs, AbstractStateRel.G S b ofs -> AbstractStateRel.G R b ofs -> False.
-
-  Lemma layer_tcomp: ksim (tensor_comp_semantics' L1 L3 sk)
-                          (tensor_comp_semantics' L2 L4 sk)
-                          (M ++ N) (R * S).
-  Proof.
-    unfold ksim in *.
-    destruct HL1 as [Hsk1 [Hmod1 H1]]. clear HL1.
-    destruct HL2 as [Hsk2 [Hmod2 H2]]. clear HL2.
-    split. eapply linkorder_refl.
-    split. apply compatible_app; (eapply compatible_trans; [ | eauto]); eauto.
-
-    exploit @tensor_compose_simulation; [exact H1 | exact H2 | .. ]; eauto. intros H.
-    eapply open_fsim_ccref. apply cc_compose_id_left.
-    unfold flip. apply cc_compose_id_right.
-    eapply compose_forward_simulations. exact H.
-
-    unfold tensor_comp_semantics'. cbn.
-    unfold layer_comp.
-
-    etransitivity.
-    {
-      apply flat_composition_simulation'. instantiate (1 := fun i => match i with true => _ | false => _ end).
-      intros [|].
-      - instantiate (1 := comp_semantics' (semantics M (skel L1) @ (K2 * K4)) (lift_layer_k L2) (skel L1)).
-        etransitivity.
-        + apply mapB_monotonicity. etransitivity.
-          * apply mapA_monotonicity. apply lift_categorical_comp1.
-          * apply mapA_comp.
-        + etransitivity.
-          * apply mapB_comp'. typeclasses eauto.
-          * eapply categorical_compose_simulation'.
-            -- apply lts_lifting_assoc.
-            -- reflexivity.
-            -- apply linkorder_refl.
-            -- auto.
-      - instantiate (1 := comp_semantics' (semantics N (skel L3) @ (K2 * K4)) (layer_comm (lift_layer_k L4)) (skel L3)).
-        etransitivity.
-        + apply mapB_monotonicity. etransitivity.
-          * apply mapB_monotonicity. etransitivity.
-            -- apply mapA_monotonicity. apply lift_categorical_comp1.
-            -- apply mapA_comp.
-          * apply mapB_comp'. typeclasses eauto.
-        + etransitivity.
-          * apply mapB_comp'. typeclasses eauto.
-          * eapply categorical_compose_simulation'.
-            -- etransitivity.
-               ++ apply map_both_monotonicity. apply lts_lifting_assoc.
-               ++ apply lts_lifting_comm.
-            -- reflexivity.
-            -- apply linkorder_refl.
-            -- auto.
-      - intros [|]; auto.
-    }
-
-    set (LX:= fun i:bool => if i then semantics M (skel L1) @ (K2 * K4) else semantics N (skel L3) @ (K2 * K4)).
-    set (LY:= fun i:bool => if i then lift_layer_k L2 else layer_comm (lift_layer_k L4)).
-    set (Lsk:= fun i:bool => if i then skel L1 else skel L3).
-    replace (flat_comp_semantics' _ sk) with (flat_comp_semantics' (fun i:bool => comp_semantics' (LX i) (LY i) (Lsk i)) sk).
-    2: {
-      subst LX  LY Lsk. cbn. f_equal. apply functional_extensionality.
-      intros [|]; reflexivity.
-    }
-
-    etransitivity. apply categorical_flat_interchangeable.
-    eapply categorical_compose_simulation'; [ | reflexivity | apply linkorder_refl | apply linkorder_refl ].
-    subst LX. rewrite <- if_rewrite with (f := fun x => x @ (K2 * K4)).
-    etransitivity. apply lift_flat_comp2. apply lifting_simulation.
-    etransitivity. 2: { apply cmodule_flat_comp_simulation. eauto. }
-    etransitivity. apply lift_flat_comp_component. cbn.
-    rewrite if_rewrite with (f := fun x => skel_extend x sk). reflexivity.
-  Qed.
-
-End TCOMP.
